iris/BioInitAt.v
@@ -159,7 +159,7 @@ Section BioInitAt.
     bio_free_tok bn -∗
     bcache_addr ↦₄ (mword_of_int 0 : mword 32) -∗
     lock_name bcache_addr "bcache"%string -∗
-    WpLock.lk_cpu_fresh bcache_addr -∗
+    WpLock.lk_cpu_ready bcache_addr -∗
     ([∗ list] k ∈ seq 0 NBUF, sl_fresh (buf_lock (bnode k)) "buffer"%string) -∗
     ([∗ list] k ∈ seq 0 NBUF, buf_raw k) -∗
     bcache_lru bhead (blist 0 NBUF) -∗
