iris/FsBoot.v
@@ -534,7 +534,7 @@ Section FsBoot.
     own_context cur_ctx -∗
     bcache_addr ↦₄ (mword_of_int 0 : mword 32) -∗
     lock_name bcache_addr "bcache"%string -∗
-    WpLock.lk_cpu_fresh bcache_addr -∗
+    WpLock.lk_cpu_ready bcache_addr -∗
     ([∗ list] k ∈ seq 0 NBUF, sl_fresh (buf_lock (bnode k)) "buffer"%string) -∗
     ([∗ list] k ∈ seq 0 NBUF,
        b_valid (bpa k) ↦₄ (mword_of_int 0 : mword 32) ∗
